Proved a simple IO example.

progs/verif_io.v
@@ -5,7 +5,7 @@ Require Import VST.floyd.proofauto.
 Require Import DeepWeb.Free.Monad.Free.
 Import MonadNotations.
 Require Import DeepWeb.Free.Monad.Common.
-(*Require Import DeepWeb.Free.Monad.Verif.*)
+Require Import DeepWeb.Free.Monad.Verif.
 
 Instance CompSpecs : compspecs. make_compspecs prog. Defined.
 Definition Vprog : varspecs. mk_varspecs prog. Defined.
@@ -14,38 +14,40 @@ Inductive IO_event : Type -> Type :=
 | ERead : IO_event int
 | EWrite (c : int) : IO_event unit.
 
+Definition read : M IO_event int := embed ERead.
+
+Definition write (c : int) : M IO_event unit := embed (EWrite c).
+
 Definition IO_itree := M IO_event unit.
 
-Definition read : IO_itree := embed ERead.
-
-Definition write (c : int) : IO_itree := embed (EWrite c).
+(* We need a layer of EqM to allow us to use the monad laws. *)
+Definition ITREE (tr : IO_itree) := EX tr' : _, !!(EquivUpToTau tr tr') && has_ext tr'.
 
 Definition putchar_spec :=
  DECLARE _putchar
-  WITH c : int, k : unit -> IO_itree
+  WITH c : int, k : IO_itree
   PRE [ _c OF tint ]
     PROP ()
     LOCAL (temp _c (Vint c))
-    SEP (has_ext (write c ;; k))
+    SEP (ITREE (write c ;; k))
   POST [ tint ]
     PROP ()
     LOCAL (temp ret_temp (Vint Int.zero))
-    SEP (has_ext k).
+    SEP (ITREE k).
 
+(* Is it okay to assume that the char is in range? *)
 Definition getchar_spec :=
  DECLARE _getchar
   WITH k : int -> IO_itree
   PRE [ ]
     PROP ()
     LOCAL ()
-    SEP (has_ext (r <- read ;; k r))
+    SEP (ITREE (r <- read ;; k r))
   POST [ tint ]
    EX i : int,
-    PROP ()
+    PROP (- two_p 7 <= Int.signed i <= two_p 7 - 1)
     LOCAL (temp ret_temp (Vint i))
-    SEP (has_ext (k i)).
-
-Parameter chars_of_Z : Z -> list int.
+    SEP (ITREE (k i)).
 
 Fixpoint write_list l : IO_itree :=
   match l with
@@ -53,17 +55,279 @@ Fixpoint write_list l : IO_itree :=
   | c :: rest => write c ;; write_list rest
   end.
 
+Definition char0 : Z := 48.
+
+Program Fixpoint chars_of_nat n { measure n } : list int :=
+  match (n / 10)%nat with
+  | O => [Int.repr (Z.of_nat n + char0)]
+  | n' => chars_of_nat n' ++ [Int.repr (Z.of_nat (n mod 10) + char0)]
+  end.
+Next Obligation.
+Proof.
+  apply (Nat.div_lt n 10); try omega.
+  destruct n; [contradiction | omega].
+Defined.
+
+Definition chars_of_Z z := chars_of_nat (Z.to_nat z).
+
+(* The function computed by print_intr *)
+Program Fixpoint intr n { measure n } : list int :=
+  match n with
+  | O => []
+  | _ => intr (n / 10) ++ [Int.repr (Z.of_nat (n mod 10) + char0)]
+  end.
+Next Obligation.
+Proof.
+  apply (Nat.div_lt n 10); try omega.
+Defined.
+
 Definition print_intr_spec :=
  DECLARE _print_intr
   WITH i : Z, tr : IO_itree
   PRE [ _i OF tuint ]
-    PROP ()
+    PROP (0 <= i <= Int.max_unsigned)
     LOCAL (temp _i (Vint (Int.repr i)))
-    SEP (has_ext (write_list (chars_of_Z i) ;; tr)
+    SEP (ITREE (write_list (intr (Z.to_nat i)) ;; tr))
   POST [ tvoid ]
     PROP ()
     LOCAL ()
-    SEP (has_ext tr).
+    SEP (ITREE tr).
+
+Definition print_int_spec :=
+ DECLARE _print_int
+  WITH i : Z, tr : IO_itree
+  PRE [ _i OF tuint ]
+    PROP (0 <= i <= Int.max_unsigned)
+    LOCAL (temp _i (Vint (Int.repr i)))
+    SEP (ITREE (write_list (chars_of_Z i) ;; tr))
+  POST [ tvoid ]
+    PROP ()
+    LOCAL ()
+    SEP (ITREE tr).
+
+Definition newline := 10.
+
+CoFixpoint read_sum n : IO_itree := write_list (chars_of_Z n);; write (Int.repr newline);;
+  c <- read;; read_sum (n + (Int.unsigned c - char0)).
+
+Definition main_itree := c <- read;; read_sum (Int.unsigned c - char0).
+
+(* Note nonstandard main_spec; in general, we probably want floyd to support
+   a version of main_spec with a starting has_ext assertion. *)
+Definition main_spec :=
+ DECLARE _main
+  WITH u : unit
+  PRE  [] PROP () LOCAL () SEP (ITREE main_itree)
+  POST [ tint ] PROP () LOCAL () SEP (TT).
 
 Definition Gprog : funspecs := ltac:(with_library prog [putchar_spec; getchar_spec;
-  print_intr_spec]).
+  print_intr_spec; print_int_spec; main_spec]).
+
+Lemma ITREE_impl : forall tr tr', EquivUpToTau tr tr' -> ITREE tr |-- ITREE tr'.
+Proof.
+  intros.
+  unfold ITREE.
+  Intros tr1; Exists tr1; entailer!.
+  etransitivity; eauto.
+  symmetry; auto.
+Qed.
+
+Lemma ITREE_ext : forall tr tr', EquivUpToTau tr tr' -> ITREE tr = ITREE tr'.
+Proof.
+  intros; apply pred_ext; apply ITREE_impl; auto.
+  symmetry; auto.
+Qed.
+
+Lemma divu_repr : forall x y,
+  0 <= x <= Int.max_unsigned -> 0 <= y <= Int.max_unsigned ->
+  Int.divu (Int.repr x) (Int.repr y) = Int.repr (x / y).
+Proof.
+  intros; unfold Int.divu.
+  rewrite !Int.unsigned_repr; auto.
+Qed.
+
+Opaque bind.
+
+Lemma write_list_app : forall l1 l2,
+  EquivUpToTau (write_list (l1 ++ l2)) (write_list l1;; write_list l2).
+Proof.
+  induction l1; simpl; intros.
+  - symmetry; apply leftId.
+  - rewrite <- bindAssoc.
+    Transparent bind.
+    simpl.
+    apply cong_bind; [reflexivity|].
+    intro; apply IHl1.
+Qed.
+
+Opaque Nat.div Nat.modulo.
+
+Lemma intr_eq : forall n, intr n =
+  match n with
+  | O => []
+  | _ => intr (n / 10) ++ [Int.repr (Z.of_nat (n mod 10) + char0)]
+  end.
+Proof.
+  intros.
+  unfold intr at 1.
+  rewrite Wf.WfExtensionality.fix_sub_eq_ext; simpl; fold intr.
+  destruct n; reflexivity.
+Qed.
+
+Lemma body_print_intr: semax_body Vprog Gprog f_print_intr print_intr_spec.
+Proof.
+  start_function.
+  forward_if (PROP () LOCAL () SEP (ITREE tr)).
+  - forward.
+    forward.
+    rewrite modu_repr, divu_repr by (omega || computable).
+    rewrite intr_eq.
+    destruct (Z.to_nat i) eqn: Hi.
+    { apply Z2Nat_inj_0 in Hi; omega. }
+    rewrite <- Hi, mod_Zmod, Z2Nat.id by omega; simpl; clear dependent n.
+    erewrite ITREE_ext
+      by (apply cong_bind with (k' := fun _ => tr); [apply write_list_app | reflexivity]).
+    change (bindM _ _) with ((write_list (intr (Z.to_nat i / 10));; write_list [Int.repr (i mod 10 + char0)]);; tr).
+    erewrite ITREE_ext by (symmetry; apply bindAssoc).
+    forward_call (i / 10, write_list [Int.repr (i mod 10 + char0)];; tr).
+    { replace (Z.to_nat i / 10)%nat with (Z.to_nat (i / 10)); [cancel|].
+      rewrite <- (Z2Nat.id i) at 1 by omega.
+      rewrite <- (div_Zdiv _ 10) by omega.
+      rewrite Nat2Z.id; auto. }
+    { split; [apply Z.div_pos; omega | apply Z.div_le_upper_bound; omega]. }
+    forward_call (Int.repr (i mod 10 + 48), tr).
+    { rewrite <- sepcon_emp at 1; apply sepcon_derives; [|cancel].
+      erewrite ITREE_ext; [apply derives_refl|].
+      unfold write_list.
+      apply cong_bind; [|reflexivity].
+      simpl.
+      replace (fun _ => Ret tt) with (fun x : unit => Ret(Event := IO_event) x)
+        by (extensionality x; destruct x; auto).
+      apply (rightId(s := write (Int.repr (i mod 10 + char0)))). }
+    entailer!.
+  - forward.
+    subst; entailer!.
+    erewrite ITREE_ext; [apply derives_refl|].
+    apply (leftId tt (fun _ => tr)).
+  - forward.
+Qed.
+
+Lemma chars_of_nat_eq : forall n, chars_of_nat n =
+  match (n / 10)%nat with
+  | O => [Int.repr (Z.of_nat n + char0)]
+  | n' => chars_of_nat n' ++ [Int.repr (Z.of_nat (n mod 10) + char0)]
+  end.
+Proof.
+  intros.
+  unfold chars_of_nat at 1.
+  rewrite Wf.WfExtensionality.fix_sub_eq_ext; simpl; fold chars_of_nat.
+  destruct (n / 10)%nat; reflexivity.
+Qed.
+
+Lemma chars_of_nat_intr : forall n, (0 < n)%nat ->
+  chars_of_nat n = intr n.
+Proof.
+  induction n using (well_founded_induction lt_wf); intro.
+  rewrite chars_of_nat_eq, intr_eq.
+  destruct n; [omega|].
+  forget (S n) as m.
+  destruct (_ / _)%nat eqn: Hdiv.
+  - rewrite mod_Zmod by omega; simpl.
+    rewrite Zmod_small; auto.
+    split; try omega.
+    apply Z2Nat.inj_lt; try omega.
+    rewrite Nat2Z.id; simpl.
+    destruct (lt_dec m 10); auto.
+    exploit (Nat.div_str_pos m 10); omega.
+  - rewrite H; auto; try omega.
+    rewrite <- Hdiv; apply Nat.div_lt; auto; omega.
+Qed.
+
+Lemma body_print_int: semax_body Vprog Gprog f_print_int print_int_spec.
+Proof.
+  start_function.
+  forward_if (PROP () LOCAL () SEP (ITREE tr)).
+  - subst.
+    forward_call (Int.repr char0, tr).
+    { unfold chars_of_Z; rewrite chars_of_nat_eq.
+      change (_ / _)%nat with O; simpl.
+      erewrite <- sepcon_emp at 1; apply sepcon_derives; [|cancel].
+      erewrite ITREE_ext; [apply derives_refl|].
+      apply cong_bind; [|reflexivity].
+      replace (fun _ => Ret tt) with (fun x : unit => Ret(Event := IO_event) x)
+        by (extensionality x; destruct x; auto).
+      apply (rightId(s := write (Int.repr char0))). }
+    entailer!.
+  - forward_call (i, tr).
+    { unfold chars_of_Z.
+      rewrite chars_of_nat_intr; [cancel|].
+      destruct (Z.to_nat i) eqn: Hi; [|omega].
+      apply Z2Nat_inj_0 in Hi; omega. }
+    entailer!.
+  - forward.
+Qed.
+
+Opaque bind.
+
+Lemma read_sum_eq : forall n, read_sum n =
+  (write_list (chars_of_Z n);; write (Int.repr newline);;
+   c <- read;; read_sum (n + (Int.unsigned c - char0))).
+Proof.
+  intro.
+  rewrite matchM; simpl.
+  rewrite <- matchM; auto.
+Qed.
+
+Lemma body_main: semax_body Vprog Gprog f_main main_spec.
+Proof.
+  start_function.
+  forward.
+  unfold main_itree.
+  rewrite <- !seq_assoc. (* Without this, forward_call gives a type error! *)
+  forward_call (fun c => read_sum (Int.unsigned c - char0)).
+  Intros c.
+  forward.
+  rewrite sign_ext_inrange by auto.
+  set (Inv := EX n : Z, EX c : int,
+    PROP (0 <= n < 1009)
+    LOCAL (temp _c (Vint c); temp _n (Vint (Int.repr n)))
+    SEP (ITREE (read_sum (n + (Int.unsigned c - char0))))).
+  unfold Swhile; forward_loop Inv break: Inv.
+  { Exists 0 c; entailer!.
+    apply derives_refl. }
+  subst Inv.
+  clear dependent c; Intros n c.
+  forward_if.
+  forward.
+  forward_if.
+  { forward.
+    Exists n c; entailer!. }
+  forward.
+  rewrite read_sum_eq.
+  rewrite <- (Int.repr_unsigned c) in H1.
+  rewrite sub_repr in H1.
+  pose proof (Int.unsigned_range c).
+  destruct (zlt (Int.unsigned c) char0).
+  { rewrite Int.unsigned_repr_eq in H1.
+    rewrite <- Z_mod_plus_full with (b := 1), Zmod_small in H1; unfold char0 in *; rep_omega. }
+  rewrite Int.unsigned_repr in H1 by (unfold char0 in *; rep_omega).
+  forward_call (n + (Int.unsigned c - char0),
+    write (Int.repr newline);; c' <- read;; read_sum (n + (Int.unsigned c - char0) + (Int.unsigned c' - char0))).
+  { entailer!.
+    rewrite <- (Int.repr_unsigned c) at 1.
+    rewrite sub_repr, add_repr; auto. }
+  { unfold char0 in *; rep_omega. }
+  forward_call (Int.repr newline, c' <- read;; read_sum (n + (Int.unsigned c - char0) + (Int.unsigned c' - char0))).
+  forward_call (fun c' => read_sum (n + (Int.unsigned c - char0) + (Int.unsigned c' - char0))).
+  Intros c'.
+  forward.
+  rewrite sign_ext_inrange by auto.
+  Exists (n + (Int.unsigned c - char0)) c'; entailer!.
+  split; [unfold char0 in *; omega|].
+  rewrite <- (Int.repr_unsigned c) at 2; rewrite sub_repr, add_repr; auto.
+  { forward.
+    Exists n c; entailer!. }
+  subst Inv.
+  Intros n c'.
+  forward.
+Qed.
